Record failed attempt

Regex/NFA/Transition.lean
@@ -454,71 +454,302 @@ theorem compile.loop.stepSet_subset (eq : compile.loop r next nfa = result)
   let ⟨h, _⟩ := step_range c eq i h''.left h''.right
   exact h
 
-inductive NFA.eval (nfa : NFA) : Set Nat → List Char → Set Nat → List Char → Prop where
-  | base : nfa.eval S cs S cs
-  | step (rest : nfa.eval (nfa.stepSet' S c) cs S' cs') : nfa.eval S (c :: cs) S' cs'
+-- inductive NFA.eval (nfa : NFA) : Set Nat → List Char → Set Nat → List Char → Prop where
+--   | base : nfa.eval S cs S cs
+--   | step (rest : nfa.eval (nfa.stepSet' S c) cs S' cs') : nfa.eval S (c :: cs) S' cs'
 
-theorem NFA.eval_prefix {nfa : NFA} (ev : nfa.eval S s S' s₂) :
+inductive NFA.eval (nfa : NFA) : Nat → List Char → Nat → List Char → Prop where
+  | base (eqi : i = j) (eqs : cs = cs') : nfa.eval i cs j cs'
+  | charStep {i j k : Nat} {c : Char} {cs cs' : List Char}
+    (h : i < nfa.nodes.size) (step : j ∈ nfa[i].charStep c) (rest : nfa.eval j cs k cs') :
+    nfa.eval i (c :: cs) k cs'
+  | εStep {i j k : Nat} {cs cs' : List Char}
+    (h : i < nfa.nodes.size) (step : j ∈ nfa[i].εStep) (rest : nfa.eval j cs k cs') :
+    nfa.eval i cs k cs'
+
+theorem NFA.eval_prefix {nfa : NFA} (ev : nfa.eval i s j s₂) :
   ∃s₁, s = s₁ ++ s₂ := by
   induction ev with
   | base => exists []
-  | @step _ c _ _ _ _ ih =>
+  | @charStep _ _ _ c _ _ _ _ _ ih =>
     let ⟨s₁', h⟩ := ih
     exists c :: s₁'
     simp [h]
+  | εStep _ _ _ ih => exact ih
 
-notation:65 nfa " ⊢ (" S ", " s ") ⟶* (" S' ", " s' ")" => NFA.eval nfa S s S' s'
+notation:65 nfa " ⊢ (" i ", " s ") ⟶* (" j ", " s' ")" => NFA.eval nfa i s j s'
+
+-- When we expand the NFA by appending nodes, the evaluation relation is preserved in the original range.
+
+theorem eval_ge_of_get_lt {nfa nfa' : NFA} (le : nfa.nodes.size ≤ nfa'.nodes.size)
+  (get_lt : ∀ {i}, (h : i < nfa.nodes.size) → nfa'[i]'(Nat.lt_of_lt_of_le h le) = nfa[i])
+  (ev : nfa ⊢ (i, s) ⟶* (j, s')) :
+  nfa' ⊢ (i, s) ⟶* (j, s') := by
+  induction ev with
+  | base eqi eqs => exact .base eqi eqs
+  | charStep h step _ ih =>
+    have eqi := get_lt h
+    exact .charStep
+      (Nat.lt_of_lt_of_le h le) (eqi.symm ▸ step) ih
+  | εStep h step _ ih =>
+    have eqi := get_lt h
+    exact .εStep
+      (Nat.lt_of_lt_of_le h le) (eqi.symm ▸ step) ih
+
+theorem eval_le_of_get_lt {nfa nfa' : NFA} (le : nfa.nodes.size ≤ nfa'.nodes.size)
+  (get_lt : ∀ {i}, (h : i < nfa.nodes.size) → nfa'[i]'(Nat.lt_of_lt_of_le h le) = nfa[i])
+  (h₁ : i < nfa.nodes.size) (h₂ : nfa.inBounds) (ev : nfa' ⊢ (i, s) ⟶* (j, s')) :
+  nfa ⊢ (i, s) ⟶* (j, s') := by
+  induction ev with
+  | base eqi eqs => exact .base eqi eqs
+  | @charStep i j _ c _ _ _ step _ ih =>
+    have eqi := get_lt h₁
+    rw [eqi] at step
+    have : j < nfa.nodes.size := show j ∈ { j | j < nfa.nodes.size } by
+      exact mem_of_mem_of_subset step ((h₂ ⟨i, h₁⟩).left c)
+    exact .charStep h₁ step (ih this)
+  | @εStep i j _ _ _ _ step _ ih =>
+    have eqi := get_lt h₁
+    rw [eqi] at step
+    have : j < nfa.nodes.size := show j ∈ { j | j < nfa.nodes.size } by
+      exact mem_of_mem_of_subset step (h₂ ⟨i, h₁⟩).right
+    exact .εStep h₁ step (ih this)
+
+theorem eval_addNode_of_eval (eq : NFA.addNode nfa node = result)
+  (ev : nfa ⊢ (i, s) ⟶* (j, s')) : result ⊢ (i, s) ⟶* (j, s') :=
+  eval_ge_of_get_lt (NFA.le_size_of_le result.property) (fun h => eq ▸ NFA.get_lt_addNode h) ev
+
+theorem eval_compile_of_eval (eq : compile.loop r next nfa = result)
+  (ev : nfa ⊢ (i, s) ⟶* (j, s')) : result ⊢ (i, s) ⟶* (j, s') :=
+  eval_ge_of_get_lt (NFA.le_size_of_le result.property) (compile.loop.get_lt eq) ev
+
+theorem eval_of_eval_addNode (eq : NFA.addNode nfa node = result)
+  (h₁ : i < nfa.nodes.size) (h₂ : nfa.inBounds)
+  (ev : result ⊢ (i, s) ⟶* (j, s')) : nfa ⊢ (i, s) ⟶* (j, s') :=
+  eval_le_of_get_lt (NFA.le_size_of_le result.property) (fun h => eq ▸ NFA.get_lt_addNode h) h₁ h₂ ev
+
+theorem eval_of_eval_compile (eq : compile.loop r next nfa = result)
+  (h₁ : i < nfa.nodes.size) (h₂ : nfa.inBounds)
+  (ev : result ⊢ (i, s) ⟶* (j, s')) : nfa ⊢ (i, s) ⟶* (j, s') :=
+  eval_le_of_get_lt (NFA.le_size_of_le result.property) (compile.loop.get_lt eq) h₁ h₂ ev
+
+-- The compiled NFA first circulates within the new nodes range,
+-- then it must go to the next node before escaping to the original range.
 
 theorem eval_to_next_of_eval (eq : compile.loop r next nfa = result)
-  -- hsはnextを含むのかな？含まない気もしてきた
-  -- そもそもstartが{result.val.start}にした方がいいのかも
-  (ev : result ⊢ (S, s) ⟶* (S', s')) (hs : S ⊆ {next} ∪ compile.loop.NewNodesRange eq)
-  (h₁ : i ∈ S') (h₂ : i < nfa.nodes.size) :
-  ∃ S'' s'', result ⊢ (S, s) ⟶* (S'', s'') ∧ next ∈ S'' := by
+  (h₁ : i ∈ compile.loop.NewNodesRange eq) (h₂ : k < nfa.nodes.size)
+  (ev : result ⊢ (i, s) ⟶* (k, s'')) :
+  ∃ s', result ⊢ (i, s) ⟶* (next, s') ∧ result ⊢ (next, s') ⟶* (k, s'') := by
   induction ev with
-  | @base S cs =>
-    exists S, cs, .base
-    have : i ∈ {next} ∪ compile.loop.NewNodesRange eq :=
-      mem_of_subset_of_mem hs h₁
-    have : i = next ∨ i ∈ compile.loop.NewNodesRange eq :=
-      mem_insert_iff.mp this
-    cases this with
-    | inl h => exact h ▸ h₁
-    | inr h =>
-      simp [compile.loop.NewNodesRange] at h
-      exact (Nat.not_lt_of_ge h.left h₂).elim
-  | @step S c cs S' cs' rest ih => sorry
+  | base eqi =>
+    simp [compile.loop.NewNodesRange] at h₁
+    exact (Nat.not_lt_of_ge h₁.left (eqi.symm ▸ h₂)).elim
+  | @charStep i j k c cs cs' h step rest ih =>
+    have mem : j ∈ {next} ∪ compile.loop.NewNodesRange eq := by
+      apply mem_of_mem_of_subset step
+      exact (compile.loop.step_range c eq i h₁.left h₁.right).left
+    cases Nat.decEq j next with
+    | isTrue eq =>
+      rw [←eq]
+      exact ⟨cs, .charStep h step (.base rfl rfl), rest⟩
+    | isFalse neq =>
+      have : j ∈ compile.loop.NewNodesRange eq := Set.mem_of_mem_insert_of_ne mem neq
+      let ⟨s', ih₁, ih₂⟩ := ih this h₂
+      exact ⟨s', .charStep h step ih₁, ih₂⟩
+  | @εStep i j k cs cs' h step rest ih =>
+    have mem : j ∈ {next} ∪ compile.loop.NewNodesRange eq := by
+      apply mem_of_mem_of_subset step
+      exact (compile.loop.step_range default eq i h₁.left h₁.right).right
+    cases Nat.decEq j next with
+    | isTrue eq =>
+      rw [←eq]
+      exact ⟨cs, .εStep h step (.base rfl rfl), rest⟩
+    | isFalse neq =>
+      have : j ∈ compile.loop.NewNodesRange eq := Set.mem_of_mem_insert_of_ne mem neq
+      let ⟨s', ih₁, ih₂⟩ := ih this h₂
+      exact ⟨s', .εStep h step ih₁, ih₂⟩
 
-theorem matches_of_eval (eq : compile.loop r next nfa = nfa') (assm : next < nfa.nodes.size)
-  (ev : nfa' ⊢ ({nfa'.val.start.val}, s) ⟶* (S', s')) (h : next ∈ S') : ∃p, s = p ++ s' ∧ r.matches ⟨p⟩ := by
-  induction r generalizing next nfa s S' s' with
-  | empty =>
-    apply compile.loop.empty eq
-    intro eq
+theorem eval_to_next_of_eval_from_start (eq : compile.loop r next nfa = result)
+  (h : k < nfa.nodes.size) (ev : result ⊢ (result.val.start, s) ⟶* (k, s'')) :
+  ∃ s', result ⊢ (result.val.start, s) ⟶* (next, s') ∧ result ⊢ (next, s') ⟶* (k, s'') := by
+  have h₁ : result.val.start.val ∈ compile.loop.NewNodesRange eq := compile.loop.start_in_NewNodesRange eq
+  exact eval_to_next_of_eval eq h₁ h ev
 
-    sorry
+inductive evalStar (eq : compile.loop (.star r) next nfa = result) : List Char → List Char → Prop where
+  | complete (eqs : s = s') : evalStar eq s s'
+  | step (evR : result ⊢ (result.val.start, s) ⟶* (result.val.start, s'')) (evRest : result ⊢ (result.val.start, s'') ⟶* (next, s'))
+    (rest : evalStar eq s'' s') : evalStar eq s s'
+
+theorem matches_prefix_of_eval (eq : compile.loop r next nfa = nfa')
+  (h₁ : next < nfa.nodes.size) (h₂ : nfa.inBounds)
+  (ev : nfa' ⊢ (nfa'.val.start, s) ⟶* (next, s')) :
+  ∃ p, s = p ++ s' ∧ r.matches ⟨p⟩ := by
+  induction r generalizing next nfa s s' with
+  | empty => sorry
   | epsilon => sorry
   | char c => sorry
-  | alternate r₁ r₂ => sorry
+  | alternate r₁ r₂ ih₁ ih₂ =>
+    apply compile.loop.alternate eq
+    intro nfa₁ start₁ nfa₂ start₂ final property eq₁ eq₂ eq₃ eq₄ eq₅ eq
+
+    have inBounds₁ := compile.loop.inBounds eq₁.symm h₁ h₂
+    have inBounds₂ :=
+      compile.loop.inBounds eq₃.symm (Nat.lt_of_lt_of_le h₁ (NFA.le_size_of_le nfa₁.property)) inBounds₁
+    have size₁ : next < nfa₁.val.nodes.size := Nat.lt_of_lt_of_le h₁ (NFA.le_size_of_le nfa₁.property)
+
+    rw [eq] at ev
+    simp at ev
+
+    cases ev with
+    | base eqi =>
+      have : final.val.start.val ≠ next := by
+        apply Nat.ne_of_gt
+        calc next
+          _ < nfa.nodes.size := h₁
+          _ ≤ nfa₂.val.nodes.size := NFA.le_size_of_le (NFA.le_trans nfa₁.property nfa₂.property)
+          _ = _ := by
+            rw [eq₅]
+            simp [NFA.addNode]
+      contradiction
+    | @charStep _ j _ c _ _ _ step =>
+      have : final.val[final.val.start].charStep c = ∅ := by
+        rw [eq₅]
+        simp [Node.charStep]
+      have : j ∈ ∅ := this ▸ step
+      exact this.elim
+    | @εStep i j k cs cs' h step rest =>
+      have : j = start₁.val ∨ j = start₂.val := by
+        subst eq₅
+        simp [Node.εStep] at step
+        exact step
+      have ev₂ : nfa₂ ⊢ (j, s) ⟶* (next, s') := by
+        apply eval_of_eval_addNode eq₅.symm _ inBounds₂ rest
+        cases this with
+        | inl h =>
+          have lt₁ : start₁ < nfa₂.val.nodes.size :=
+            Nat.lt_of_lt_of_le start₁.isLt (NFA.le_size_of_le nfa₂.property)
+          simp [h, lt₁]
+        | inr h => simp [h]
+      cases this with
+      | inl step₁ =>
+        have ev₁ : nfa₁ ⊢ (j, s) ⟶* (next, s') := by
+          apply eval_of_eval_compile eq₃.symm _ inBounds₁ ev₂
+          simp [step₁]
+        let ⟨p, eqs, m₁⟩ := ih₁ eq₁.symm h₁ h₂ (eq₂ ▸ step₁ ▸ ev₁)
+        exact ⟨p, eqs, .alternateLeft m₁⟩
+      | inr step₂ =>
+        let ⟨p, eqs, m₂⟩ := ih₂ eq₃.symm size₁ inBounds₁ (eq₄ ▸ step₂ ▸ ev₂)
+        exact ⟨p, eqs, .alternateRight m₂⟩
   | concat r₁ r₂ ih₁ ih₂ =>
     apply compile.loop.concat eq
     intro nfa₂ nfa₁ property eq₂ eq₁ eq
 
-    -- ここでS₁はnfa₂.val.start.valを含むような奴が実はとれる
-    have ev₁ : ∃S₁ s₂_s', nfa₁ ⊢ ({nfa₁.val.start.val}, s) ⟶* (S₁, s₂_s') := sorry
-    let ⟨S₁, s₂_s', ev₁⟩ := ev₁
-    have h₁ : nfa₂.val.start.val ∈ S₁ := sorry
-    have ⟨s₁, eqs₁, m₁⟩ := ih₁ eq₁.symm nfa₂.val.start.isLt ev₁ h₁
+    have inBounds₂ := compile.loop.inBounds eq₂.symm h₁ h₂
+    have inBounds₁ := compile.loop.inBounds eq₁.symm nfa₂.val.start.isLt inBounds₂
 
-    have ev₂ : nfa₂ ⊢ ({nfa₂.val.start.val}, s₂_s') ⟶* (S', s') := sorry
-    have h₂ : next ∈ S' := sorry
-    have ⟨s₂, eqs₂, m₂⟩ := ih₂ eq₂.symm assm ev₂ h₂
+    rw [eq] at ev
+    simp at ev
+    have : next < nfa₂.val.nodes.size := Nat.lt_of_lt_of_le h₁ (NFA.le_size_of_le nfa₂.property)
+    let ⟨s₂s', ev₁, ev'⟩ := eval_to_next_of_eval_from_start eq₁.symm this ev
+    let ⟨s₁, eqs₁, m₁⟩ := ih₁ eq₁.symm nfa₂.val.start.isLt inBounds₂ ev₁
 
-    have eqs : s = s₁ ++ s₂ ++ s' := by
-      rw [List.append_assoc]
-      exact eqs₂ ▸ eqs₁
+    have ev₂ : nfa₂ ⊢ (nfa₂.val.start, s₂s') ⟶* (next, s') :=
+      eval_of_eval_compile eq₁.symm nfa₂.val.start.isLt inBounds₂ ev'
+    let ⟨s₂, eqs₂, m₂⟩ := ih₂ eq₂.symm h₁ h₂ ev₂
 
-    exact ⟨s₁ ++ s₂, eqs, .concat ⟨s₁ ++ s₂⟩ ⟨s₁⟩ ⟨s₂⟩ r₁ r₂ rfl m₁ m₂⟩
-  | star r => sorry
+    exact ⟨s₁ ++ s₂, by simp [eqs₁, eqs₂], .concat ⟨s₁ ++ s₂⟩ ⟨s₁⟩ ⟨s₂⟩ r₁ r₂ rfl m₁ m₂⟩
+  | star r ih =>
+    apply compile.loop.star eq
+    intro placeholder start compiled nodes final isLt isLt' property'
+      eq₁ eq₂ eq₃ eq₄ eq₅ eq'
+
+    have placeholder.inBounds : placeholder.val.inBounds := by
+      intro i
+      cases Nat.lt_or_ge i nfa.nodes.size with
+      | inl lt =>
+        have : placeholder.val[i] = nfa[i] := by
+          simp [eq₁, NFA.get_lt_addNode lt]
+        rw [this]
+        exact Node.inBounds_of_inBounds_of_le (h₂ ⟨i, lt⟩) (NFA.le_size_of_le placeholder.property)
+      | inr ge =>
+        have : i < nfa.nodes.size + 1 := by
+          have : i < placeholder.val.nodes.size := i.isLt
+          simp [eq₁, NFA.addNode] at this
+          exact this
+        have : i = nfa.nodes.size := Nat.eq_of_ge_of_lt ge this
+        have : placeholder.val[i] = .fail := by
+          simp [eq₁, this]
+        rw [this]
+        simp
+
+    have evStar : evalStar eq s s' := by
+      have ev : final ⊢ (final.start, s) ⟶* (next, s') := by
+        subst eq'
+        exact ev
+      have split : final[final.start.val] = .split compiled.val.start next := by
+        subst eq₅
+        simp [NFA.eq_get, eq₄]
+      cases ev with
+      | base _ eqs => exact .complete eqs
+      | charStep _ step => simp [split, Node.charStep] at step
+      | @εStep i j k s s' _ step rest =>
+        simp [split, Node.εStep] at step
+        -- NOTE: It's actually possible to step away from the node range of `star r`.
+        -- For example, when we compile `(a*)*`, we can escape the region of `(a*)` to the first node of
+        -- `(a*)*` by taking an εStep, and then go back to the first node by another εStep.
+        -- Such a case cannot be handled by this setup.
+        sorry
+    induction evStar with
+    | complete eqs => exact ⟨[], by simp [eqs], .starEpsilon rfl⟩
+    | @step s s'' s' evR evRest rest ih' =>
+      let ⟨p, eqsr, m⟩ : ∃ p, s = p ++ s'' ∧ r.matches ⟨p⟩ := by
+        suffices compiled ⊢ (compiled.val.start, s) ⟶* (start, s'') from
+          ih eq₃.symm start.isLt placeholder.inBounds this
+        have evR : nfa' ⊢ (start, s) ⟶* (start, s'') := by
+          have : nfa'.val.start.val = start.val := by
+            subst eq' eq₅
+            rfl
+          exact this ▸ evR
+        -- ここでevRの第一歩について場合分けするのduplicationじゃないか？後で考える
+        sorry
+      let ⟨p', eqsr', m'⟩ := ih' evRest
+      exact ⟨p ++ p', by simp [eqsr, eqsr'], .starConcat _ _ _ _ rfl m m'⟩
+
+theorem mwe (x : α) (f : α → Array Nat) (g : α → Fin (f x).size) (eq : f x = t) :
+  (f x)[g x] = t[(g x).cast (by rw [eq])] := by
+  aesop_subst eq
+  simp_all only [getElem_fin, Fin.coe_cast]
+
+-- theorem matches_of_eval (eq : compile.loop r next nfa = nfa') (assm : next < nfa.nodes.size)
+--   (ev : nfa' ⊢ ({nfa'.val.start.val}, s) ⟶* (S', s')) (h : next ∈ S') : ∃p, s = p ++ s' ∧ r.matches ⟨p⟩ := by
+--   induction r generalizing next nfa s S' s' with
+--   | empty =>
+--     apply compile.loop.empty eq
+--     intro eq
+
+--     sorry
+--   | epsilon => sorry
+--   | char c => sorry
+--   | alternate r₁ r₂ => sorry
+--   | concat r₁ r₂ ih₁ ih₂ =>
+--     apply compile.loop.concat eq
+--     intro nfa₂ nfa₁ property eq₂ eq₁ eq
+
+--     -- ここでS₁はnfa₂.val.start.valを含むような奴が実はとれる
+--     have ev₁ : ∃S₁ s₂_s', nfa₁ ⊢ ({nfa₁.val.start.val}, s) ⟶* (S₁, s₂_s') := sorry
+--     let ⟨S₁, s₂_s', ev₁⟩ := ev₁
+--     have h₁ : nfa₂.val.start.val ∈ S₁ := sorry
+--     have ⟨s₁, eqs₁, m₁⟩ := ih₁ eq₁.symm nfa₂.val.start.isLt ev₁ h₁
+
+--     have ev₂ : nfa₂ ⊢ ({nfa₂.val.start.val}, s₂_s') ⟶* (S', s') := sorry
+--     have h₂ : next ∈ S' := sorry
+--     have ⟨s₂, eqs₂, m₂⟩ := ih₂ eq₂.symm assm ev₂ h₂
+
+--     have eqs : s = s₁ ++ s₂ ++ s' := by
+--       rw [List.append_assoc]
+--       exact eqs₂ ▸ eqs₁
+
+--     exact ⟨s₁ ++ s₂, eqs, .concat ⟨s₁ ++ s₂⟩ ⟨s₁⟩ ⟨s₂⟩ r₁ r₂ rfl m₁ m₂⟩
+--   | star r => sorry
 
 end NFA
